# CFG to CNF

## CFG: The language generated by CFG is called Context Free Grammar
----

## Simplification:
---------------

## CNF: Chomskey Normal Form :-
---------------------------

A→BC [variables]  
A→ a  [Terminal]

A,B,C Represent Variables. a represents terminal

- If there exist terminal at right side, then there must be only one terminal
- If there exist variables at right side, Then there must be exactly TWO variables
- No ε rules (S→ε) is allowed except START variable → ε 
- START variables cannot exist in the right of any product rules.


## CNF Conversion:
---------------

## EXAMPLE: 1

```
S→ ASA|aB
A→ B  | S
B→ b  | ε 
```

### STEP 1: Add new start variable
-------

   

```
L → S 
S→ ASA|aB
A→ B  | S
B→ b  | ε 
```

### STEP 2: Remove ε rules except Start Variable pointing to ε 
-------
 
#### B→ ε Removal: 
--------------
1. Remove ε
2. Find out the ε containing variables in RIGHT side of other Rules
3. ADD those variables with the ε with those Rules

```
L → S
S→ ASA|aB | a    [aB → aε == a]
A→ B  | S | ε    [B→ε == ε]
B→ b             [Remove ε from the Variable]
```

#### A→ ε Removal:
--------------

```
L → S
S→ ASA | aB | a | AS | SA | S [ASA → εSε  == S]
                              [ASA → εSA ==  SA]    
                              [ASA → ASε == AS]

A→ B  | S  [Remove ε from the Variable]
B→ b
```

### STEP 3: unit rules (V → P)[right side single variable] Removal
-------

#### Self Removal: S→ S
--------------------

```
L → S
S→ ASA | aB | a | AS | SA [Removed S]
A→ B | S
B→ b
```

#### A → B Removal:
---------------
```
L → S
S→ ASA | aB | a | AS | SA [Removed S]
A→ b | S [Removed B]
         [A→ B → b == A → b]
B→ b
```

#### A→ S Removal:
--------------
```
L → S
S→ ASA | aB | a | AS | SA 
A→ b |ASA | aB | a | AS | SA  [Removed S]
                              [A→ S → ASA | aB | a | AS | SA]
B→ b
```

#### L → S Removal:
-------------------
```
L → ASA | aB | a | AS | SA     [L → S → ASA | aB | a | AS | SA]
S→ ASA | aB | a | AS | SA 
A→ b |ASA | aB | a | AS | SA  
B→ b
```

### STEP 4: Proper Form Conversion
-------

```
L → AP | QB | a | AS | SA     [L → S → ASA | aB | a | AS | SA]
P    → SA
Q    → a
S    → AP | QB | a | AS | SA 
A    → b |AP | QB | a | AS | SA  
B     → b
```

**We made two new Rules here:**

* in CNF there can be Maximum TWO variables but as We can see we have "ASA" 3 Variables. To reduced it to TWO variables We made the Below Rule  

___P → SA___

* in CNF nonTerminal(Variables) and Terminal can't be together, Also Maximum two variables can be declared simultaneously.
To fix this issue, we made the Below Rule.


___Q → a___

The END!  
This the Chomollokko Normal Form 

## Example 2:
----------

```
A → BAB | B | ε 
B → 00 | ε 
```

### STEP 1: Add new start variable
-------
```
S → A
A → BAB | B | ε 
B → 00 | ε 
```

### STEP 2: Remove ε rules except Start Variable pointing to ε
-------
#### A → ε Removal:
----------------
```
S → A | ε
A → BAB | B | BB 
B → 00 | ε
```

#### B→ ε Removal:
--------------
```
S → A | ε
A → BAB | B | BB | BA | AB | A  [(B → ε == ε , BB → εε) == ε] 
                                [There supposed to be an ε . But in previous step we removed ε from B. So we don't need to add it again]
B → 00 
```

### STEP 3: unit rules (V → P)[right side single variable] Removal
-------
#### Self Removal: A → A
--------------------
```
S → A | ε
A → BAB | B | BB | BA | AB 
B → 00 
```

#### A → B Removal:
---------------
```
S → A | ε
A → BAB | 00 | BB | BA | AB
B → 00
```

#### S → A Removal:
---------------
```
S → BAB | 00 | BB | BA | AB | ε 
A → BAB | 00 | BB | BA | AB
B → 00
```

### STEP 4: Proper Form Conversion
------------------------------

```
S → BP | QQ | BB | BA | AB | ε
P → AB
Q → 0
A → BP | QQ | BB | BA | AB
B → QQ
```

The END!

## Example 3:
----------
```
S→ aXbX
X → aY | bY | ε
Y → X | c
```

### CNF Conversion:
---------------

#### STEP 1: Add new start variable
-------------------------------
```
L → S
S→ aXbX
X → aY | bY | ε
Y → X | c
```

#### STEP 2: Remove ε rules except Start Variable pointing to ε
-----------------------------------------------------------
##### X → ε Removal:
---------------
```
L → S
S → aXbX | aXb | abX | ab
X → aY | bY
Y → X | c | ε 
```

##### Y → ε Removal:
----------------
```
L → S
S    → aXbX | aXb | abX | ab
X    → aY | bY | a | b
Y    → X | c
```

#### STEP 3: unit rules
-------------------

##### Self Removal:
-------------
>**Nothing to remove**


##### Single Variables Removal:
--------------------------

###### Y → X Removal
--------------
```
L    → S
S    → aXbX | aXb | abX | ab
X    → aY | bY | a | b
Y    → aY | bY | a | b | c
```

###### L → S Removal
-----------------
```
L    → aXbX | aXb | abX | ab
S    → aXbX | aXb | abX | ab
X    → aY | bY | a | b
Y    → aY | bY | a | b | c
```

#### STEP 4: Proper Conversion
--------------------------

```
L    → PQ | PB | AQ | AB

A    → a
B    → b

P    → AX [aX]
Q    → BX [bX]

S    → PQ | PB | AQ | AB
X    → AY | BY | a | b
Y    → AY | BY | a |b | c
```

The END

## Example 5:
----------

```
S → aX | bY | b | ZZc
X → Yaa| abZ| ε 
Y → bXXb | ab | cZ
Z → a | b | XZ | ε 
```

### CNF Conversion:
---------------

#### STEP 1:
-------
```
U → S
S → aX | bY | b | ZZc
X → Yaa| abZ| ε 
Y → bXXb | ab | cZ
Z → a | b | XZ | ε 
```

#### STEP 2: ε Removal
-----------------

##### X → ε Removal
--------------
```
U → S
S → aX | bY | b | ZZc | a
X → Yaa| abZ
Y → bXXb | ab | cZ | bXb | bb
Z → a | b | XZ | ε | Z
```

##### Z → ε Removal:
---------------

```
U → S
S → aX | bY | b | ZZc | a | Zc | c
X → Yaa| abZ | ab
Y → bXXb | ab | cZ | bXb | bb | c
Z → a | b | XZ | Z | X
```

#### STEP 3: Unit Removal
---------------------

##### Self Removal:
-------------

###### Z → Z Removal:
---------------

```
U → S
S → aX | bY | b | ZZc | a | Zc | c
X → Yaa| abZ | ab
Y → bXXb | ab | cZ | bXb | bb | c
Z → a | b | XZ | X
```

##### Single Variable Removal:
------------------------

###### Z → X Removal:
----------------
```
U → S
S → aX | bY | b | ZZc | a | Zc | c
X → Yaa| abZ | ab
Y → bXXb | ab | cZ | bXb | bb | c
Z → a | b | XZ | Yaa| abZ | ab
```

###### U → S Removal:
---------------

```
U → aX | bY | b | ZZc | a | Zc | c

S → aX | bY | b | ZZc | a | Zc | c
X → Yaa| abZ | ab
Y → bXXb | ab | cZ | bXb | bb | c
Z → a | b | XZ | Yaa| abZ | ab
```

#### STEP 4: Proper Conversion
--------------------------

```
U → AX | BY | b | DC | a | ZC | c
A → a
B → b
C → c
D → ZZ
S → AX | BY | b | DC | a | ZC | c
X → YE| FZ | AB
E → AA
F → AB
Y → GH | AB | CZ | GB | BB | c
G → BX
H → XB
Z → a | b | XZ | YE| FZ | AB
```